# 作业四

## 1、证明

1. $\forall$x$\forall$yPxy   Hyp
2. $\forall$a$\forall$bPab  将x,y分别替换为a,b
3. $\forall$y$\forall$xPyx  将a,b分别替换为y,x

    Q.E.D.

## 2、证明

### 2.1

Lemma 1:{a$\rightarrow$b,b$\rightarrow$c}$\vdash$a$\rightarrow$c  显然成立。

#### (1)

先证$\rightarrow$:

1. $\lnot$$\forall$x$\lnot$$\alpha$$\rightarrow$$\lnot$($\lnot$$\alpha$)<sup>x</sup><sub>t</sub><p align="right">AX2.7.2</p>
2. $\lnot$$\forall$x$\lnot$$\beta$$\rightarrow$$\lnot$($\lnot$$\beta$)<sup>x</sup><sub>t</sub><p align="right">AX2.7.2</p>
3. $\lnot$($\lnot$$\alpha$)<sup>x</sup><sub>t</sub>$\rightarrow$($\lnot$($\lnot$$\alpha$)<sup>x</sup><sub>t</sub>$\vee$$\lnot$($\lnot$$\beta$)<sup>x</sup><sub>t</sub>)<p align="right">AX1.22.4</p>
4. $\lnot$($\lnot$$\beta$)<sup>x</sup><sub>t</sub>$\rightarrow$($\lnot$($\lnot$$\alpha$)<sup>x</sup><sub>t</sub>$\vee$$\lnot$($\lnot$$\beta$)<sup>x</sup><sub>t</sub>)<p align="right">AX1.22.5</p>
5. $\lnot$$\forall$x$\lnot$$\alpha$$\rightarrow$($\lnot$($\lnot$$\alpha$)<sup>x</sup><sub>t</sub>$\vee$$\lnot$($\lnot$$\beta$)<sup>x</sup><sub>t</sub>)<p align="right">Lemma 1</p>
6. $\lnot$$\forall$x$\lnot$$\beta$$\rightarrow$($\lnot$($\lnot$$\alpha$)<sup>x</sup><sub>t</sub>$\vee$$\lnot$($\lnot$$\beta$)<sup>x</sup><sub>t</sub>)<p align="right">Lemma 1</p>
7. $\lnot$$\forall$x$\lnot$$\alpha$$\vee$$\lnot$$\forall$x$\lnot$$\beta$$\rightarrow$($\lnot$($\lnot$$\alpha$)<sup>x</sup><sub>t</sub>$\vee$$\lnot$($\lnot$$\beta$)<sup>x</sup><sub>t</sub>)<p align="right">AX1.22.6</p>
8. $\lnot$$\forall$x$\lnot$$\alpha$$\vee$$\lnot$$\forall$x$\lnot$$\beta$$\rightarrow$($\lnot$$\forall$x$\lnot$($\alpha$$\vee$$\beta$))<p align="right">Ded.+Gen.</p>
9. $\exist$x$\alpha$$\vee$$\exist$x$\beta$$\rightarrow$($\exist$x($\alpha$$\vee$$\beta$))<p align="right">rewrite</p>

再证$\leftarrow$:同理可证。

综上，$\vdash$$\exist$x$\alpha$$\vee$$\exist$x$\beta$ $\leftrightarrow$$\exist$x ($\alpha$$\vee$$\beta$)<p align="right">Q.E.D.</p>

#### (2)

1. $\forall$x$\alpha$$\rightarrow$($\alpha$)<sup>x</sup><sub>t</sub><p align="right">AX2.7.2</p>
2. $\forall$x$\beta$$\rightarrow$($\beta$)<sup>x</sup><sub>t</sub><p align="right">AX2.7.2</p>
3. ($\alpha$)<sup>x</sup><sub>t</sub>$\rightarrow$(($\alpha$)<sup>x</sup><sub>t</sub>$\vee$($\beta$)<sup>x</sup><sub>t</sub>)<p align="right">AX1.22.4</p>
4. ($\beta$)<sup>x</sup><sub>t</sub>$\rightarrow$(($\alpha$)<sup>x</sup><sub>t</sub>$\vee$($\beta$)<sup>x</sup><sub>t</sub>)<p align="right">AX1.22.5</p>
5. $\forall$x$\alpha$$\rightarrow$(($\alpha$)<sup>x</sup><sub>t</sub>$\vee$($\beta$)<sup>x</sup><sub>t</sub>)<p align="right">Lemma 1</p>
6. $\forall$x$\beta$$\rightarrow$(($\alpha$)<sup>x</sup><sub>t</sub>$\vee$($\beta$)<sup>x</sup><sub>t</sub>)<p align="right">Lemma 1</p>
7. $\forall$x$\alpha$$\vee$$\forall$x$\beta$$\rightarrow$(($\alpha$)<sup>x</sup><sub>t</sub>$\vee$($\beta$)<sup>x</sup><sub>t</sub>)<p align="right">AX1.22.6</p>
8. $\forall$x$\alpha$$\vee$$\forall$x$\beta$$\rightarrow$($\forall$x($\alpha$$\vee$$\beta$))<p align="right">Ded.+Gen.</p>
<p align="right">Q.E.D.</p>

### 2.2

Lemma 1:{a$\rightarrow$b,b$\rightarrow$c}$\vdash$a$\rightarrow$c  显然成立。

#### (1)

1. $\lnot$$\forall$x$\lnot$($\alpha$$\wedge$$\beta$)$\rightarrow$$\lnot$($\lnot$($\alpha$$\wedge$$\beta$))<sup>x</sup><sub>t</sub><p align="right">AX2.7.2</p>
2. $\lnot$($\lnot$($\alpha$$\wedge$$\beta$)<sup>x</sup><sub>t</sub>)$\rightarrow$$\lnot$($\lnot$(($\alpha$)<sup>x</sup><sub>t</sub>$\wedge$($\beta$)<sup>x</sup><sub>t</sub>))<p align="right">def</p>
3. $\lnot$$\forall$x$\lnot$($\alpha$$\wedge$$\beta$)$\rightarrow$$\lnot$($\lnot$(($\alpha$)<sup>x</sup><sub>t</sub>$\wedge$($\beta$)<sup>x</sup><sub>t</sub>))<p align="right">Lemma 1</p>
4. $\lnot$$\forall$x$\lnot$($\alpha$$\wedge$$\beta$)$\rightarrow$$\lnot$($\forall$x$\lnot$$\alpha$)$\wedge$($\forall$x$\lnot$$\beta$)<p align="right">Ded.+Gen.</p>
5. $\exist$x($\alpha$$\wedge$$\beta$)$\rightarrow$(($\exist$x$\alpha$)$\wedge$($\exist$x$\beta$))<p align="right">rewrite</p>
<p align="right">Q.E.D.</p>

#### (2)

先证$\rightarrow$:同2.2（1）证法易证。

再证$\leftarrow$:

1. $\forall$x$\alpha$$\wedge$$\forall$x$\beta$$\rightarrow$($\alpha$<sup>x</sup><sub>t</sub>)$\wedge$($\beta$<sup>x</sup><sub>t</sub>)<p align="right">AX2.7.2</p>
2. ($\alpha$<sup>x</sup><sub>t</sub>)$\wedge$($\beta$<sup>x</sup><sub>t</sub>)$\rightarrow$($\alpha$$\wedge$$\beta$)<sup>x</sup><sub>t</sub><p align="right">def</p>
3. $\forall$x$\alpha$$\wedge$$\forall$x$\beta$$\rightarrow$($\alpha$$\wedge$$\beta$)<sup>x</sup><sub>t</sub><p align="right">Lemma 1</p>
4. $\forall$x$\alpha$$\wedge$$\forall$x$\beta$$\rightarrow$$\forall$x($\alpha$$\wedge$$\beta$)<p align="right">Ded.+Gen.</p>

综上，$\vdash$$\forall$x($\alpha$$\wedge$$\beta$)$\leftrightarrow$ $\forall$x$\alpha$$\wedge$$\forall$x$\beta$<p align="right">Q.E.D.</p>
